\documentclass{article}
\usepackage{bm}
\usepackage{amsmath,amsfonts,amssymb,amsthm}
\usepackage{newpxtext} 
\usepackage{relsize}
\usepackage{comment}
\usepackage{booktabs}
\usepackage{stackengine} 
\usepackage{adjustbox}
\usepackage{mathtools}
\usepackage{graphicx} % Required for inserting images

\title{Calculus Assignment 3}
\author{Erik Paskalev}
\date{September 2024}

\begin{document}

\maketitle

\section{\normalfont Prove the formula}

\begin{equation}
(t^2)' = 2t
\end{equation}

\section*{\normalfont using the product rule and the fact that $t' = 1$}

\section*{Proof:}

\begin{equation}
(t^2)' = (t*t)' = t'*t + t*t' = t + t = 2t
\end{equation}

\section{\normalfont Using the product rule (and the other rules), take the derivative of the following functions:}

\section*{Answer:}

\begin{equation}
\begin{split}
te^t & = e^t + te^t = (t+1)e^t \\
t^2e^t & = 2te^2 + t^2e^t = (t^2 + 2t)e^t \\
3 + 4^t - t^2 8^t & = 4 - 2t8^t - t^2 8^t ln(8) = 4 - 8^t t(2 + tln(8))\\
2t^3 2^t 3^t & = (2t^3)' 2^t 3^t + 2t^3(2^t 3^t)' = 6t^2 2^t 3^t + 2t^3(2^t 3^t ln(2) + 2^t 3^t ln(3)) = \\ 
& = (3 + tln(2) + tln(3))2t^2 2^t 3^t = (3 + tln(6))t^2 2^{t+1} 3^t \\
t^4 e^t 2^t & = 4t^3 e^t 2^t + t^4(e^t 2^t + e^t 2^t ln(2)) = (4 + t + tln(2))t^3 e^t 2^t
\end{split}
\end{equation}

\section{\normalfont Prove the formula $(t^4)' = 4t^3$ by using the product rule three times.}

\section*{Proof:}

\begin{equation}
\begin{split}
(t^4)' & = (t*t*t*t)' = (t)'t^3 + t(t*t*t)' = t^3 + t((t)'t^2 + t(t*t)') = \\
& = t^3 + t(t^2 + t((t)'t + t(t)')) = t^3 + t(t^2 + t(t + t)) = \\ 
& = t^3 + t^3 + t^3 + t^3 = 4t^3
\end{split}
\end{equation}

\section{\normalfont Assuming $p$ to be an integer, prove that $ln(t^p) = p ln(t)$ using the property $ln(a Â· b)$ = $ln(a) + ln(b)$.}

\section*{Proof:}

\begin{equation}
ln(t^p) = ln(\underbrace{t*t*t*...*t}_{\text{p times}}) = \underbrace{ln(t) + ln(t) + ln(t) + ... + ln(t)}_{\text{p times}} = pln(t)
\end{equation}

\section{\normalfont Show that $(a^t)' = ln(a)a^t$ assuming that you know that $(e^{bt})' = be^{bt}$ for all values of $b$}

\section*{Proof:}

\begin{equation}
(a^t)' = (e^{ln(a^t)})' = (e^{ln(a)t})' = ln(a)e^{ln(a)t} = ln(a)e^{ln(a^t)} = ln(a)a^t
\end{equation}

\end{document}
